src/ReactorModel/Execution/State.lean
@@ -1,0 +1,20 @@
+import ReactorModel.Execution.Context
+
+structure Execution.State (ι υ) [Value υ] where
+  rtr : Reactor ι υ
+  ctx : Context ι
+
+namespace Execution.State 
+
+variable {ι υ} [Value υ]
+
+structure isNextTag (s : State ι υ) (g : Time.Tag) : Prop where
+  mem : g ∈ s.rtr.scheduledTags
+  lower : s.ctx.time < g
+  upper : ∀ g' ∈ s.rtr.scheduledTags, s.ctx.time < g' → g ≤ g'
+
+theorem isNextTag_unique {s : State ι υ} {g₁ g₂ : Time.Tag} :
+  (s.isNextTag g₁) → (s.isNextTag g₂) → g₁ = g₂ :=
+  sorry
+
+end Execution.State 
